src/relation_semantic.v
@@ -184,13 +184,14 @@ with eval_expr_list_to (arch : architecture)
         eval_expr_to arch fprog ctxt hd val_hd ->
         eval_expr_list_to arch fprog ctxt tl val_tl ->
         eval_expr_list_to arch fprog ctxt (ECons hd tl) (linearize_list_value val_hd val_tl)
-with eval_vars_to (arch : architecture)
-    : prog -> list (ident * @cst_or_int Z) -> seq var -> list cst_or_int -> Prop :=
+with eval_bvars_to (arch : architecture)
+    : prog -> list (ident * @cst_or_int Z) -> seq bvar -> list cst_or_int -> Prop :=
+    (* TODO *)
 with check_deq (arch : architecture)
     : prog -> list (ident * @cst_or_int Z) -> deq -> Prop :=
-    | CDEqn : forall fprog ctxt vars e val,
+    | CDEqn : forall fprog ctxt (vars : seq bvar) e val,
         eval_expr_to arch fprog ctxt e val ->
-        eval_vars_to arch fprog ctxt vars val ->
+        eval_bvars_to arch fprog ctxt vars val ->
         check_deq arch fprog ctxt (Eqn vars e false)
     | CDLoop : forall fprog ctxt i start_e start_i end_e end_i deqs opt,
         eval_arith_expr ctxt start_e start_i ->
@@ -211,8 +212,8 @@ with eval_node_to (arch : architecture)
     : prog -> p -> p -> def_i -> option nat -> list (@cst_or_int Z) -> list (@cst_or_int Z) -> Prop :=
     | EVTSingle :
         forall fprog in_names temp_names out_names in_values out_values eqns ctxt,
-        eval_vars_to arch fprog ctxt (map (fun v => Var (VD_ID v)) in_names) in_values ->
-        eval_vars_to arch fprog ctxt (map (fun v => Var (VD_ID v)) out_names) out_values ->
+        eval_bvars_to arch fprog ctxt (map (fun v => (VD_ID v, nil)) in_names) in_values ->
+        eval_bvars_to arch fprog ctxt (map (fun v => (VD_ID v, nil)) out_names) out_values ->
         check_deq_list arch fprog ctxt eqns ->
         eval_node_to arch fprog in_names out_names (Single temp_names eqns) None in_values out_values
     | EVTMultiple :
